

## MIDTERM EXAMINATION

Academic year 2012-2013, Semester 2

Duration: 90 minutes

<b>SUBJECT:</b> <b>Differential Equations</b>	
Acting Chair of Department of Mathematics	Lecturer:
Signature:	Signature:
Associate Prof. Nguyen Dinh	Associate Prof. Pham Huu Anh Ngoc

**Instructions:**

- *Each student is allowed a scientific calculator and a maximum of two double-sided sheets of reference material (size A4 or similar), stapled together and marked with their name and ID. All other documents and electronic devices are forbidden.*

**Question 1.** a) (10 marks) Show that the differential equation

$$(e^{2y} - y \cos(xy))dx + (2xe^{2y} - x \cos(xy) + 2y)dy = 0,$$

is exact.

b) (15 marks) Solve the equation given in a).

**Question 2.** (25 marks) Find the solution to the initial value problem

$$x(x+1)y' + xy = 1, \quad x \in (0, \infty); \quad y(e) = 1.$$

**Question 3.** a) (10 marks) Solve the differential equation

$$y'' - 3y' = 0.$$

b) (15 marks) Find the general solution of the differential equation

$$y'' - 3y' = 8e^{3x} + 4 \sin x.$$

**Question 4.** (10 marks) a) Show that  $y_1(x) = x$  is a solution of the differential equation

$$x^2 y'' - 3xy' + 3y = 0.$$

b) (15 marks) Solve the differential equation

$$x^2 y'' - 3xy' + 3y = 2x^4 e^x.$$

END.

# SOLUTIONS:

**Question 1.** a) Let

$$M(x, y) = e^{2y} - y \cos(xy); \quad N(x, y) = 2xe^{2y} - x \cos(xy) + 2y.$$

Thus the given equation is exact.

$$\frac{\partial M}{\partial y}(x, y) = \frac{\partial N}{\partial x}(x, y) = 2e^{2y} - \cos(xy) + xy \sin(xy).$$

b) The general solution is given by

$$xe^{2y} - \sin(xy) + y^2 = C.$$

**Question 2.** The given equation is written as

$$y' + \frac{1}{x+1}y = \frac{1}{x(x+1)}, \quad x > 0.$$

The integrating factor is given by  $I(x) = x + 1$ . Thus, we get

$$(x+1)y' + y = \frac{1}{x}, \quad x > 0.$$

This gives

$$\frac{d}{dx}[y(1+x)] = \ln x + C, \quad x > 0.$$

Therefore, the general solution is

$$y(x) = \frac{\ln x + C}{x+1}.$$

Since  $y(e) = 1$ , the particular solution is  $y(x) = \frac{\ln x + e}{x+1}$ .

**Question 3.**

a) The general solution of the homogeneous equation is

$$y(x) = c_1 + c_2 e^{3x}.$$

b) A particular solution of  $y'' - 3y' = 8e^{3x} + 4 \sin x$  is  $y_p(x) = (8/3)e^{3x}x - (2/5) \sin x + (6/5) \cos x$ . Thus the general solution of the equation  $y'' - 3y' = 8e^{3x} + 4 \sin x$ , is given by

$$y(x) = (8/3)e^{3x}x - (2/5) \sin x + (6/5) \cos x + c_1 + c_2 e^{3x}.$$

**Question 4.** a) So easy.

b) The general solution is given by

$$y(x) = 2e^x(x^2 - x) + c_1 x^3 + c_2 x.$$